# (APPENDIX) Appendix {-}

# Variance/covariance rules {#appendix-rules}



-  **Rule 1**

If $C$ is constant, then

$$
Var\left(C\right) = 0
$$

-  **Rule 2**

If $X_{1}$ and $X_{2}$ are independent, then

$$
Var\left(X_{1} + X_{2}\right) =
Var\left(X_{1}\right) + Var\left(X_{2}\right)
$$

Consequence of **Rule 1** and **Rule 2**:

$$
Var\left(X + C\right) = Var\left(X\right)
$$

-  **Rule 3**

If $X_{1}$ and $X_{2}$ are independent, then

$$
Var\left(X_{1} - X_{2}\right) =
Var\left(X_{1}\right) + Var\left(X_{2}\right)
$$


-  **Rule 4**

If $a$ is any number, 

$$
Var\left(aX\right) = a^2 Var\left(X\right)
$$


-  **Rule 5**

$$
Cov(X, X) = Var(X)
$$

-  **Rule 6**

$$
Cov\left(X_{1}, X_{2}\right) = Cov\left(X_{2}, X_{1}\right)
$$

-  **Rule 7**

If $C$ is constant, then

$$
Cov\left(X, C\right) = 0
$$

-  **Rule 8**

$$
Cov\left(X_{1} + X_{2}, X_{3}\right) = Cov\left(X_{1}, X_{3}\right) + Cov\left(X_{2}, X_{3}\right)  
$$

-  **Rule 9**

$$
Cov\left(X_{1} - X_{2}, X_{3}\right) = Cov\left(X_{1}, X_{3}\right) - Cov\left(X_{2}, X_{3}\right)  
$$

Consequence of **Rule 6**, **Rule 8**, and **Rule 9**:

$$
Cov\left(X_{1}, X_{2} \pm X_{3}\right) = Cov\left(X_{1}, X_{2}\right) \pm Cov\left(X_{1}, X_{3}\right)  
$$
-  **Rule 10**

If $a$ is any number, 

$$
Cov\left(a X_{1}, X_{2}\right) = a Cov\left(X_{1}, X_{2}\right) =  Cov\left(X_{1}, a X_{2}\right)  
$$

-  **Rule 11**

If $X_{1}$ and $X_{2}$ are independent, then

$$
Cov\left(X_{1}, X_{2}\right) = 0
$$

-  **Rule 12**

For *any* two variables $X_{1}$ and $X_{2}$:

$$
Var(aX_{1} + bX_{2}) = 
    a^2Var(X_{1}) + b^2Var(X_{2}) + 2abCov(X_{1}, X_{2})
$$



# LISREL notation {#appendix-lisrel}
